\section{Control}

\subsection{Actuator model}
$$
\textbf{mech:  }
K_r^{-1} \tau = K_t i_a
\qquad
\textbf{electr:  }
v_a = R_ai_a + K_v \dot{q}_m
\ , \
v_a = G_vV_c
\qquad
;
\qquad
\left[ K_r q = q_m \right]
$$

%\vspace*{5pt}
\subsubsection{Velocity generator: }
$$
\omega_m = \frac{G_v}{k_v} v_c'
\qquad
F = F_v K_r K_t R_a^{-1} K_v K_r 
\qquad
u = K_r K_t R_a^{-1} G_v v_c
\qquad
\qquad
$$
$$
u = \tau + F\dot{q} 
\implies
\tau = K_r K_t R_a^{-1} (G_vv_c - K_vK_r\dot{q})
\qquad
v_c \approx G_v^{-1} K_v K_r \dot{q}
$$

%\vspace*{5pt}
\subsubsection{Torque generator: }
$$
c_m \approx \frac{k_t}{k_i} ( v_c' - \frac{k_v}{G_v}\omega_m)
$$



\subsection{Decentralized joint control}
$$
\tau = K_r \tau_m
\qquad
q = K_r^{-1}q_m
\qquad
B(q) = \bar{B} + \Delta B(q) \quad 
%(\bar{B} = \textit{diag. and const})
$$

$$
K_r^{-1} \bar{B} K_r^{-1} \ddot{q}_m + 
\underbrace{
 K_r^{-1}\Delta B(q) K_r^{-1} \ddot{q}_m +
 K_r^{-1}C(q, \dot{q})K_r^{-1}\dot{q}_m +  K_r^{-1}g(q)
}_{d}
+  
\underbrace{K_r^{-1}F_vK_r^{-1}}_{F_m}\dot{q}_m = \tau_m \\
$$

$$
\textbf{t.f. motor:  } M(s) = \frac{k_m}{s(1+T_ms)}
\qquad \quad
%\text{gain const: }
k_m = \frac{1}{k_v}
\ , \
%\text{time const: }
T_m = \frac{R_a I}{k_t k_v}
$$

$$
\textbf{PI control:  } C(s) = K_c \frac{1+sT_c}{s}
\qquad
\left[ \ K_c \equiv K_p, T_c \equiv T_p \ \| \ K_c \equiv K_v, \ \cdots \ \right]
$$

\subsubsection{Position feedback}
$$
\text{forward path: } \quad G(s) = \frac{k_m K_p(1+sT_p)}{s^2(1+sT_m)}
\implies
\begin{cases}
	\text{\times} & T_p < T_m \\
	\text{\checkmark} & T_p > T_m \\
	\text{\checkmark} \, \rotatebox[origin=c]{90}{\gg} & T_p \gg T_m \\
\end{cases}
$$


\subsection{Centralized joint control}

$$
\text{current controlled} 
\implies 
i_a = G_i v_c
\implies 
u = K_rK_tG_iv_c = \tau
$$

$$
x = 
\begin{bmatrix}q \\ \dot{q} \end{bmatrix}
\implies
\dot{x} = 
\begin{bmatrix}
\dot{q} \\
B^{-1}(q) \left[ u - C(q, \dot{q})\dot{q} - F\dot{q} - g(q) \right]
\end{bmatrix}
\qquad
x_{eq} \iff \dot{x} = 0 \iff 
\begin{cases}
	\dot{q} = 0 \\
	\bar{u} = g(\bar{q})
\end{cases}
$$

\subsubsection{PD control with gravity compensation}
$$
V(\dot{q}, e) = \frac{1}{2}\dot{q}^TB(q)\dot{q} + \frac{1}{2}e^TK_Pe > 0 \qquad \forall \dot{q},e \neq 0
\qquad \qquad
e \triangleq q_d - q
$$

$$
\dot{V} = \dot{q}^TB(q)\ddot{q} + \frac{1}{2}\dot{q}^T\dot{B}(q)\dot{q} - \dot{q}^TK_Pe
\qquad
u = g(q) + K_p e - K_d \dot{q}
$$
\vspace*{-15pt}

\subsubsection{Inverse dynamics (feedback linearization)}

$$
B(q)\ddot{q} + n(q, \dot{q}) = \tau = u
\quad
\overset{F.L.}{\implies}
\quad
u \triangleq B(q)y + n(q, \dot{q})
\quad
\implies
\quad
\ddot{q} = y
$$

$$
\text{PD control: } \qquad
y \triangleq -K_P q - K_D \dot{q} + r
\quad , \quad
r \triangleq \ddot{q}_d + K_P q_d + K_D \dot{q}_d
$$

$$
\left[
\quad
\overset{\ddot{q} = y}{\implies}
\ddot{q} + K_P q + K_D \dot{q} = r
\quad \implies \quad
\ddot{e} + K_D \dot{e} + K_P e = 0
\quad
\right]
$$

$$
\implies \quad
\bm{y} = \bm{K_p}(\bm{q}_d - \bm{q}) + \bm{K_d}(\dot{\bm{q}}_d - \dot{\bm{q}}) + \ddot{\bm{q}}_d
$$

$$
\left[
\ 
%\textit{to decouple: }
\quad 
K_P = diag\{\omega_{n1}^2, \ \dots, \ \omega_{nn}^2\}
\quad
K_D = diag\{2\zeta\omega_{n1}, \ \dots, \ 2\zeta\omega_{nn}^2\}
\quad
\right]
$$




\subsection{Operational space control}

\subsubsection{PD with gravity compensation}

$$
e \triangleq x_d - x
\qquad 
u = g(q) + J_A^T(q)K_P e - J_A^T(q)K_P K_D J_A(q)\dot{q}
$$

$$
V(\dot{q}, e) = \frac{1}{2}\dot{q}^TB(q)\dot{q} + \frac{1}{2}e^TK_Pe > 0 \qquad \forall \dot{q},e \neq 0
$$

$$
\text{at equilibrium } \quad \dot{x} = (\dot{q}, \ddot{q}) = 0
\quad \implies \quad
-J_A^T(q)K_P e = 0
$$


\subsubsection{Inverse dynamics (feedback linearization)}
$$
\dot{x} = J_A(q)\dot{q} \quad \implies \quad \ddot{x} = \dot{J}_A(q)\ddot{q} + \dot{J}_A(q, \dot{q})\dot{q}
$$

$$
u \triangleq B(q)y + n(q, \dot{q})
\ \implies \
\ddot{q} = y
\quad \implies \quad
y \triangleq J_{A}^{-1}(q)\bigl(\ddot{x}_{d}+K_{D}\dot{e}+K_{P}e-\dot{J}_{A}(q,\dot{q})\dot{q}\bigr)
$$



\section{Control of the interaction}
$$
B(q)\ddot{q} + n(q, \dot{q}) = u - \underbrace{J^T(q) h}_{interaction}
\implies
\text{PD with gravity comp. } \ 
J_A^T(q)K_P e = J^T(q) h
$$

$$
h_A = T_A^T(x) K T_A(x) dx = K_A(x)(x-x_e)
\implies
e = K_P^{-1} K_A(x) (x-x_e)
$$

\begin{gather*}
x_\infty = (I - K_P^{-1}K_A(x))^{-1}(x_d + K_P^{-1}K_A(x)x_e)
\  \quad
h_{A \infty} = (I+ K_A(x)K_P^{-1})^{-1}K_A(x)(x_d-x_e)
\end{gather*}